\documentclass[12pt]{article}
\usepackage{fullpage,nicefrac,amsmath}
% \usepackage{mathpazo}
% \usepackage{amsfonts}

\newcommand{\N}{\mathbb{N}}
\newcommand{\Z}{\mathbb{Z}}
\newcommand{\Q}{\mathbb{Q}}
\newcommand{\R}{\mathbb{R}}

\begin{document}
\section*{Performance Evaluation Math Notes}
  \begin{enumerate}
    \item Why z-transform?
      \begin{enumerate}
        \item $6g_{n} - 5g_{n-1} + g_{n-2} = 6(\frac{1}{5})^n, n = 2, 3, 4, ..., g_{0} = 0, g_{1} = \frac{6}{5}$
          \begin{eqnarray*}
            6\sum_{n=2}^{\infty}{g_{n}z^{n}} - 5\sum_{n=2}^{\infty}{g_{n-1}z^{n}} + \sum_{n=2}^{\infty}{g_{n-2}z^{n}} &=& 6\sum_{n=2}^{\infty}{(\frac{1}{5})^{n}z^{n}} \\
            6\sum_{n=2}^{\infty}{g_{n}z^{n}} - 5z\sum_{n=2}^{\infty}{g_{n-1}z^{n-1}} + z^2\sum_{n=2}^{\infty}{g_{n-2}z^{n-2}} &=& 6\sum_{n=2}^{\infty}{(\frac{z}{5})^{n}} \\
            6(G(z) - g_{0} - g_{1}z) - 5z(G(z) - g_{0}) + z^2G(z) &=& \frac{6z^2}{5(5-z)} \\
            G(z)(z - 2)(z - 3) - \frac{36z}{5} &=& \frac{6z^2}{5(5-z)} \\
          \end{eqnarray*}
          \begin{eqnarray*}
            G(z) &=& \frac{6z(6 - z)}{(2 - z)(3 - z)(5 - z)} \\
                 &=& \frac{z(6 - z)}{5(1 - \frac{z}{2})(1 - \frac{z}{3})(1 - \frac{z}{5})} \\
                 &=& \frac{8}{1 - \frac{z}{2}} + \frac{-9}{1 - \frac{z}{3}} + \frac{1}{1 - \frac{z}{5}} \\
                 &=& 8\sum_{n=0}^{\infty}(\frac{1}{2})^nz^n - 9\sum_{n=0}^{\infty}(\frac{1}{3})^nz^n + \sum_{n=0}^{\infty}(\frac{1}{5})^nz^n \\
            g(z) &=& 8(\frac{1}{2})^n - 9(\frac{1}{3})^n + (\frac{1}{5})^n
          \end{eqnarray*}
        \item $a_{n+1} = 2a_{n} + 3^n + 5n, n = 1, 2, 3, ..., a_{0} = -3$
          \begin{eqnarray*}
            \sum_{n=0}^{\infty}{a_{n+1}z^{n}} &=& 2\sum_{n=0}^{\infty}{a_{n}z^{n}} + \sum_{n=0}^{\infty}3^{n}z^{n} + 5\sum_{n=0}^{\infty}{nz^{n}} \\
            \frac{A(z) - a_{0}}{z} &=& 2A(z) + \frac{1}{1 - 3z} + \frac{5z}{(1 - z)^2} \\
            A(z) + 3 &=& 2zA(z) + \frac{z}{1 - 3z} + \frac{5z^2}{(1 - z) ^ 2} \\
            A(z) &=& \frac{-3}{1 - 2z} + \frac{z}{(1 - 2z)(1 - 3z)} + \frac{5z^2}{(1 - 2z)(1 - z)^2} \\
            &=& \frac{-3}{1 - 2z} + \frac{1}{1 - 3z} - \frac{1}{1 - 2z} - \frac{5}{(1 - z)^2} + \frac{5}{1 - 2z} \\
            &=& \frac{1}{1 - 2z} + \frac{1}{1 - 3z} - \frac{5}{(1 - z)^2} \\
            &=& \frac{1}{1 - 2z} + \frac{1}{1 - 3z} - \frac{5z}{(1 - z)^2} - \frac{5}{1 - z} \\
            &=& \sum_{n=0}^{\infty}2^{n}z^{n} + \sum_{n=0}^{\infty}3^{n}z^{n} - 5\sum_{n=0}^{\infty}nz^{n} - 5\sum_{n=0}^{\infty}z^{n} \\
          \end{eqnarray*}
          \begin{eqnarray*}
            a_{n} &=& 2^{n} + 3^{n} - 5n - 5
          \end{eqnarray*}
      \end{enumerate}
    \item Poisson process Def. B to A:
      \begin{eqnarray*}
        P_{0}(t + h) &=& P(N(t + h) = 0) \\
                     &=& P(N(t) = 0, N(t + h) - N(t) = 0) \\
                     &=& P_{0}(t)(1 - \lambda h + o(h))
      \end{eqnarray*}
      For $h > 0$, $\frac{P_{0}(t + h) - P_{0}(t)}{h} = -\lambda P_{0}(t) + \frac{o(h)}{h}$. \\
      Let $h \rightarrow 0, \frac{dP_{0}(t)}{dt} = -\lambda P_{0}(t) \Rightarrow P_{0}(t) = -e^{-\lambda t}$. \\
      Let $n \geq 1$ be an arbitrary integer and assume $P[N(t + s) - N(s) = m] = e^{-\lambda t}\frac{(\lambda t)^{m}}{m!}$ is true for $1, 2, ..., n - 1$. \\
      \begin{eqnarray*}
      \Rightarrow P_{n}(t + h) &=& \sum_{k=0}^{n}(\text{exactly } k \text{ events in } [0, t]\text{, exactly } n - k \text{ events in } (t, t + h]) \\
      &=& \sum_{k=0}^{n}P_{k}(t)P_{n-k}(h) \\
      &=& P_{n}(t)P_{0}(h) + P_{n-1}(t)P_{1}(h) + o(h) \\
      &=& P_{n}(1 - \lambda h) + P_{n-1}(t)\cdot \lambda h + o(h)
      \end{eqnarray*}
      For $h > 0$, \\
      $\frac{P_{n}(t + h) - P_{n}(t)}{h} = -\lambda P_{n}(t) + \lambda P_{n-1}(t) + \frac{o(h)}{h}$. \\
      Taking $h \rightarrow 0$, we get \\
      $\frac{dP_{n}(t)}{dt} = \lambda P_{n}(t) + \lambda P_{n-1}(t)$, \\
      $\Rightarrow P_{n}(t) = e^{-\lambda t}\frac{(\lambda t)^n}{n!}$
  \end{enumerate}
\end{document}
